theories/Operational/Awkernel/MinimalProjection.v
@@ -15,11 +15,13 @@ From RocqSched Require Import Operational.Common.OSSchedulerViewContract.
 From RocqSched Require Import Operational.Common.OSHandoffContract.
 From RocqSched Require Import Operational.Common.OSCandidateSourceContract.
 From RocqSched Require Import Operational.Common.OSAdmissibleCandidateSourceContract.
+From RocqSched Require Import Operational.Common.OSSchedulerRelationContract.
 From RocqSched Require Import Refinement.OSCausalityTheorem.
 From RocqSched Require Import Refinement.OSSchedulerViewTheorem.
 From RocqSched Require Import Refinement.OSHandoffTheorem.
 From RocqSched Require Import Refinement.OSCandidateSourceTheorem.
 From RocqSched Require Import Refinement.OSAdmissibleCandidateSourceTheorem.
+From RocqSched Require Import Refinement.OSSchedulerRelationTheorem.
 From RocqSched Require Import Refinement.OSRefinementTheorem.
 From RocqSched Require Import Operational.Common.ProjectionLemmas.
 From RocqSched Require Import Operational.Common.ProjectionInvariants.
@@ -106,6 +108,18 @@ Definition awk_local_admissible_candidate_source_adapter_contract :=
 
 Definition awk_local_strong_admissible_candidate_source_adapter_contract :=
   @os_local_strong_admissible_candidate_source_adapter_contract AwkernelState.
+
+Definition awk_labeled_concrete_single_cpu_scheduler_relation_contract :=
+  @labeled_concrete_single_cpu_scheduler_relation_contract AwkernelState.
+
+Definition awk_labeled_concrete_top_m_scheduler_relation_contract :=
+  @labeled_concrete_top_m_scheduler_relation_contract AwkernelState.
+
+Definition awk_local_single_cpu_scheduler_relation_adapter_contract :=
+  @os_local_single_cpu_scheduler_relation_adapter_contract AwkernelState.
+
+Definition awk_local_top_m_scheduler_relation_adapter_contract :=
+  @os_local_top_m_scheduler_relation_adapter_contract AwkernelState.
 
 Definition awk_adapter_contract :=
   @os_multicore_adapter_contract AwkernelState.
