theories/Operational/Common/OSSchedulerRelationContract.v
@@ -1,0 +1,135 @@
+From Stdlib Require Import List Bool Arith.
+From RocqSched Require Import Foundation.Base.
+From RocqSched Require Import Semantics.Schedule.
+From RocqSched Require Import Abstractions.SchedulingAlgorithm.Interface.
+From RocqSched Require Import Abstractions.SchedulingAlgorithm.SchedulerBridge.
+From RocqSched Require Import Abstractions.SchedulingAlgorithm.TopMInterface.
+From RocqSched Require Import Abstractions.SchedulingAlgorithm.TopMSchedulerBridge.
+From RocqSched Require Import Multicore.Common.MultiCoreBase.
+From RocqSched Require Import Multicore.Common.Admissibility.
+From RocqSched Require Import Operational.Common.OSProjectionInterface.
+From RocqSched Require Import Operational.Common.ConcreteExecution.
+From RocqSched Require Import Operational.Common.Projection.
+From RocqSched Require Import Operational.Common.OSLocalAdapterContract.
+From RocqSched Require Import Operational.Common.OSCandidateSourceContract.
+
+Definition projected_scheduler_relation_schedule
+    {CState : Type}
+    {P : OSLabeledProjection CState}
+    {m : nat}
+    (ex : labeled_concrete_execution P m) : Schedule :=
+  project_schedule (osl_to_op_trace P (lce_trace ex)).
+
+Record labeled_concrete_single_cpu_scheduler_relation_contract
+    {CState : Type}
+    {P : OSLabeledProjection CState}
+    (jobs : JobId -> Job)
+    (spec : GenericSchedulingAlgorithm)
+    (candidates_of : CandidateSource)
+    (ex : labeled_concrete_execution P 1) : Prop :=
+  mkLabeledConcreteSingleCPUSchedulerRelationContract {
+    lcssrc_cpu0_follows_choose :
+      forall t,
+        projected_scheduler_relation_schedule ex t 0 =
+        spec.(choose)
+          jobs
+          1
+          (projected_scheduler_relation_schedule ex)
+          t
+          (projected_candidate_list jobs 1 ex candidates_of t);
+    lcssrc_other_cpus_idle :
+      forall t c, 0 < c ->
+        projected_scheduler_relation_schedule ex t c = None;
+  }.
+
+Arguments lcssrc_cpu0_follows_choose
+  {CState P jobs spec candidates_of ex} _ _.
+Arguments lcssrc_other_cpus_idle
+  {CState P jobs spec candidates_of ex} _ _ _ _.
+
+Record labeled_concrete_top_m_scheduler_relation_contract
+    {CState : Type}
+    {P : OSLabeledProjection CState}
+    (jobs : JobId -> Job)
+    (m : nat)
+    (spec : GenericTopMSchedulingAlgorithm)
+    (candidates_of : CandidateSource)
+    (ex : labeled_concrete_execution P m) : Prop :=
+  mkLabeledConcreteTopMSchedulerRelationContract {
+    lctmsrc_cpu_follows_choose_top_m :
+      forall t c,
+        projected_scheduler_relation_schedule ex t c =
+        if c <? m then
+          nth_error
+            (choose_top_m
+               spec
+               jobs
+               m
+               (projected_scheduler_relation_schedule ex)
+               t
+               (projected_candidate_list jobs m ex candidates_of t))
+            c
+        else
+          None;
+  }.
+
+Arguments lctmsrc_cpu_follows_choose_top_m
+  {CState P jobs m spec candidates_of ex} _ _ _.
+
+Record os_local_single_cpu_scheduler_relation_adapter_contract
+    {CState : Type}
+    (P : OSLabeledProjection CState)
+    (spec : GenericSchedulingAlgorithm)
+    (candidates_of : CandidateSource)
+    (jobs : JobId -> Job)
+    (adm : admissible_cpu) : Type :=
+  mkOSLocalSingleCPUSchedulerRelationAdapterContract {
+    olssrac_base :
+      os_local_candidate_source_adapter_contract
+        P
+        candidates_of
+        jobs
+        adm
+        1;
+    olssrac_relation :
+      labeled_concrete_single_cpu_scheduler_relation_contract
+        jobs
+        spec
+        candidates_of
+        (olac_execution (olcsac_base olssrac_base));
+  }.
+
+Arguments olssrac_base
+  {CState P spec candidates_of jobs adm} _.
+Arguments olssrac_relation
+  {CState P spec candidates_of jobs adm} _.
+
+Record os_local_top_m_scheduler_relation_adapter_contract
+    {CState : Type}
+    (P : OSLabeledProjection CState)
+    (spec : GenericTopMSchedulingAlgorithm)
+    (candidates_of : CandidateSource)
+    (jobs : JobId -> Job)
+    (adm : admissible_cpu)
+    (m : nat) : Type :=
+  mkOSLocalTopMSchedulerRelationAdapterContract {
+    oltsrac_base :
+      os_local_candidate_source_adapter_contract
+        P
+        candidates_of
+        jobs
+        adm
+        m;
+    oltsrac_relation :
+      labeled_concrete_top_m_scheduler_relation_contract
+        jobs
+        m
+        spec
+        candidates_of
+        (olac_execution (olcsac_base oltsrac_base));
+  }.
+
+Arguments oltsrac_base
+  {CState P spec candidates_of jobs adm m} _.
+Arguments oltsrac_relation
+  {CState P spec candidates_of jobs adm m} _.
